@prefix : <http://www.semanticweb.org/fnunezc/ontologies/2023/3/SpanishWineOntology#> .
@prefix owl: <http://www.w3.org/2002/07/owl#> .
@prefix rdf: <http://www.w3.org/1999/02/22-rdf-syntax-ns#> .
@prefix xml: <http://www.w3.org/XML/1998/namespace> .
@prefix xsd: <http://www.w3.org/2001/XMLSchema#> .
@prefix rdfs: <http://www.w3.org/2000/01/rdf-schema#> .
@base <http://www.semanticweb.org/fnunezc/ontologies/2023/3/SpanishWineOntology#> .

<http://www.semanticweb.org/fnunezc/ontologies/2023/3/SpanishWineOntology> rdf:type owl:Ontology ;
                                                                            <http://purl.org/dc/elements/1.1/creator> "Francisco Luis Nu√±ez Camacho" ;
                                                                            <http://purl.org/dc/elements/1.1/description> "The Spanish Wine Ontology is an ontology that models the concepts and relationships related to the production, characteristics, and consumption of wine from Spain. It provides a formal and standardized representation of wine-related knowledge, including wineries, wine varieties, regions, vintages, ratings, prices, and other relevant properties." ;
                                                                            <http://purl.org/dc/elements/1.1/questions> """- What is the highest price of a fortified wine?
- What is the highest rating given to a white wine?
- How many wines with a vintage prior to the year 2010 have a rating higher than 4?
- Are there wines without vintage in Ribera del Duero?""" ;
                                                                            <http://purl.org/dc/elements/1.1/title> "Spanish Wine Ontology" .

#################################################################
#    Annotation properties
#################################################################

###  http://purl.org/dc/elements/1.1/creator
<http://purl.org/dc/elements/1.1/creator> rdf:type owl:AnnotationProperty .


###  http://purl.org/dc/elements/1.1/description
<http://purl.org/dc/elements/1.1/description> rdf:type owl:AnnotationProperty .


###  http://purl.org/dc/elements/1.1/questions
<http://purl.org/dc/elements/1.1/questions> rdf:type owl:AnnotationProperty .


###  http://purl.org/dc/elements/1.1/title
<http://purl.org/dc/elements/1.1/title> rdf:type owl:AnnotationProperty .


###  http://swrl.stanford.edu/ontologies/3.3/swrla.owl#isRuleEnabled
<http://swrl.stanford.edu/ontologies/3.3/swrla.owl#isRuleEnabled> rdf:type owl:AnnotationProperty .


###  http://www.w3.org/2000/01/rdf-schema#sameAs
rdfs:sameAs rdf:type owl:AnnotationProperty .


#################################################################
#    Object Properties
#################################################################

###  http://www.semanticweb.org/fnunezc/ontologies/2023/3/SpanishWineOntology#madeWith
:madeWith rdf:type owl:ObjectProperty ;
          rdfs:domain :Wine ;
          rdfs:range :GrapeVariety ;
          rdfs:comment "This property relates a wine to the grape variety used in its production. It specifies the grape variety or varieties that were used in making a particular wine." .


###  http://www.semanticweb.org/fnunezc/ontologies/2023/3/SpanishWineOntology#producedBy
:producedBy rdf:type owl:ObjectProperty ;
            rdfs:domain :Wine ;
            rdfs:range :Winery ;
            rdfs:comment "This property relates a wine to the winery or producer that made it. It specifies the name of the winery or producer that made a particular wine." .


#################################################################
#    Data properties
#################################################################

###  http://www.semanticweb.org/fnunezc/ontologies/2023/3/SpanishWineOntology#hasAgingTime
:hasAgingTime rdf:type owl:DatatypeProperty ,
                       owl:FunctionalProperty ;
              rdfs:domain :Wine ;
              rdfs:range xsd:integer .


###  http://www.semanticweb.org/fnunezc/ontologies/2023/3/SpanishWineOntology#hasAlcoholicContent
:hasAlcoholicContent rdf:type owl:DatatypeProperty ,
                              owl:FunctionalProperty ;
                     rdfs:domain :Wine ;
                     rdfs:range xsd:float ;
                     rdfs:comment "Indicates the percentage of alcohol by volume (ABV) in a wine. This property provides important information about the strength of a wine and can help consumers make informed decisions about consumption. The ABV can vary depending on several factors such as grape variety, winemaking technique, and climate." .


###  http://www.semanticweb.org/fnunezc/ontologies/2023/3/SpanishWineOntology#hasRating
:hasRating rdf:type owl:DatatypeProperty ,
                    owl:FunctionalProperty ;
           rdfs:domain :Wine ;
           rdfs:range xsd:float ;
           rdfs:comment "This data property represents the rating of a wine on a scale from 0 to 5, where 0 is the lowest rating and 5 is the highest rating. The value of this property is a float." .


#################################################################
#    Classes
#################################################################

###  http://www.semanticweb.org/fnunezc/ontologies/2023/3/SpanishWineOntology#BiologicalAgeing
:BiologicalAgeing rdf:type owl:Class ;
                  rdfs:subClassOf :FortifiedWine ;
                  rdfs:comment "This class represents a type of fortified wine that has undergone biological ageing, a process where a layer of yeast grows on the surface of the wine, protecting it from oxidation and giving it a distinct flavor profile. Examples include fino and manzanilla." .


###  http://www.semanticweb.org/fnunezc/ontologies/2023/3/SpanishWineOntology#FortifiedWine
:FortifiedWine rdf:type owl:Class ;
               rdfs:subClassOf [ owl:intersectionOf ( :Wine
                                                      [ rdf:type owl:Restriction ;
                                                        owl:onProperty :hasAlcoholicContent ;
                                                        owl:someValuesFrom [ rdf:type rdfs:Datatype ;
                                                                             owl:onDatatype xsd:float ;
                                                                             owl:withRestrictions ( [ xsd:minInclusive "15.0"^^xsd:float
                                                                                                    ]
                                                                                                  )
                                                                           ]
                                                      ]
                                                    ) ;
                                 rdf:type owl:Class
                               ] ;
               rdfs:comment "Subclass of Wine representing a wine that has had additional spirits added to it." ;
               rdfs:sameAs "https://dbpedia.org/page/Fortified_wine"^^xsd:anyURI .


###  http://www.semanticweb.org/fnunezc/ontologies/2023/3/SpanishWineOntology#GrapeVariety
:GrapeVariety rdf:type owl:Class ;
              rdfs:comment "Class representing the variety of grape used to produce a wine." .


###  http://www.semanticweb.org/fnunezc/ontologies/2023/3/SpanishWineOntology#OxidizingAging
:OxidizingAging rdf:type owl:Class ;
                rdfs:subClassOf :FortifiedWine ;
                rdfs:comment "This class represents a type of fortified wine that has undergone oxidizing ageing, a process where the wine is exposed to air, leading to a darker color and a nutty flavor. Examples include amontillado and oloroso." .


###  http://www.semanticweb.org/fnunezc/ontologies/2023/3/SpanishWineOntology#PrioratRed
:PrioratRed rdf:type owl:Class ;
            rdfs:subClassOf :RedWine ;
            rdfs:comment "A subclass of RedWine that is produced in the Priorat region of Catalonia, Spain and is known for its bold and full-bodied flavor profile." .


###  http://www.semanticweb.org/fnunezc/ontologies/2023/3/SpanishWineOntology#RedGrapes
:RedGrapes rdf:type owl:Class ;
           rdfs:subClassOf :GrapeVariety ;
           rdfs:comment "A class that represents red grape varieties used in winemaking. Subclass of GrapeVariety." .


###  http://www.semanticweb.org/fnunezc/ontologies/2023/3/SpanishWineOntology#RedWine
:RedWine rdf:type owl:Class ;
         rdfs:subClassOf :Wine ;
         rdfs:comment "A subclass of Wine that is made from red grapes and is typically fermented with the grape skins and seeds, giving it its characteristic color and tannins. Subclasses include PrioratRed, RiojaRed, RiveraDelDueroRed, and ToroRed." .


###  http://www.semanticweb.org/fnunezc/ontologies/2023/3/SpanishWineOntology#RiasBaixasWhite
:RiasBaixasWhite rdf:type owl:Class ;
                 rdfs:subClassOf :WhiteWine ;
                 rdfs:comment "A subclass of WhiteWine that is produced in the Rias Baixas region of Galicia, Spain and is known for its crisp and acidic flavor profile." .


###  http://www.semanticweb.org/fnunezc/ontologies/2023/3/SpanishWineOntology#RiojaCrianza
:RiojaCrianza rdf:type owl:Class ;
              rdfs:subClassOf :RiojaRed ;
              rdfs:comment "This class represents a type of Rioja red wine that has been aged for a minimum of two years, with at least one year in oak barrels." .


###  http://www.semanticweb.org/fnunezc/ontologies/2023/3/SpanishWineOntology#RiojaRed
:RiojaRed rdf:type owl:Class ;
          rdfs:subClassOf :RedWine ;
          rdfs:comment "A subclass of RedWine that is produced in the Rioja region of Spain and is known for its balanced flavor profile and aging potential." .


###  http://www.semanticweb.org/fnunezc/ontologies/2023/3/SpanishWineOntology#RiojaReserva
:RiojaReserva rdf:type owl:Class ;
              rdfs:subClassOf :RiojaRed ;
              rdfs:comment "This class represents a type of Rioja red wine that has been aged for a minimum of three years, with at least one year in oak barrels." .


###  http://www.semanticweb.org/fnunezc/ontologies/2023/3/SpanishWineOntology#RiveraDelDueroRed
:RiveraDelDueroRed rdf:type owl:Class ;
                   rdfs:subClassOf :RedWine ;
                   rdfs:comment "A subclass of RedWine that is produced in the Ribera del Duero region of Spain and is known for its full-bodied and fruity flavor profile." .


###  http://www.semanticweb.org/fnunezc/ontologies/2023/3/SpanishWineOntology#RoseWine
:RoseWine rdf:type owl:Class ;
          rdfs:subClassOf :Wine ;
          rdfs:comment "A subclass of Wine that has a pink color and is typically made by allowing the grape skins to come into contact with the juice for a short period of time." .


###  http://www.semanticweb.org/fnunezc/ontologies/2023/3/SpanishWineOntology#RuedaWhite
:RuedaWhite rdf:type owl:Class ;
            rdfs:subClassOf :WhiteWine ;
            rdfs:comment "A subclass of WhiteWine that is produced in the Rueda region of Spain and is known for its light and refreshing flavor profile." .


###  http://www.semanticweb.org/fnunezc/ontologies/2023/3/SpanishWineOntology#SparklingWine
:SparklingWine rdf:type owl:Class ;
               rdfs:subClassOf :Wine ;
               rdfs:comment "A subclass of Wine that has high levels of carbon dioxide, resulting in bubbles." .


###  http://www.semanticweb.org/fnunezc/ontologies/2023/3/SpanishWineOntology#SweetWine
:SweetWine rdf:type owl:Class ;
           rdfs:subClassOf :Wine ;
           rdfs:comment "A subclass of Wine that has a higher level of residual sugar than other types of wine, resulting in a sweet taste." .


###  http://www.semanticweb.org/fnunezc/ontologies/2023/3/SpanishWineOntology#ToroRed
:ToroRed rdf:type owl:Class ;
         rdfs:subClassOf :RedWine ;
         rdfs:comment "A subclass of RedWine that is produced in the Toro region of Spain and is known for its high alcohol content and bold flavor profile." .


###  http://www.semanticweb.org/fnunezc/ontologies/2023/3/SpanishWineOntology#WhiteGrapes
:WhiteGrapes rdf:type owl:Class ;
             rdfs:subClassOf :GrapeVariety ;
             rdfs:comment "A class that represents white grape varieties used in winemaking. Subclass of GrapeVariety." .


###  http://www.semanticweb.org/fnunezc/ontologies/2023/3/SpanishWineOntology#WhiteWine
:WhiteWine rdf:type owl:Class ;
           rdfs:subClassOf :Wine ;
           rdfs:comment "A subclass of Wine that is made from white or green grapes and is typically fermented without the grape skins, resulting in a lighter color and less tannins. Subclasses include RiasBaixasWhite and RuedaWhite." .


###  http://www.semanticweb.org/fnunezc/ontologies/2023/3/SpanishWineOntology#Wine
:Wine rdf:type owl:Class ;
      rdfs:subClassOf [ rdf:type owl:Restriction ;
                        owl:onProperty :hasRating ;
                        owl:someValuesFrom [ rdf:type rdfs:Datatype ;
                                             owl:intersectionOf ( [ rdf:type rdfs:Datatype ;
                                                                    owl:onDatatype xsd:float ;
                                                                    owl:withRestrictions ( [ xsd:minInclusive "0.0"^^xsd:float
                                                                                           ]
                                                                                         )
                                                                  ]
                                                                  [ rdf:type rdfs:Datatype ;
                                                                    owl:onDatatype xsd:float ;
                                                                    owl:withRestrictions ( [ xsd:maxInclusive "5.0"^^xsd:float
                                                                                           ]
                                                                                         )
                                                                  ]
                                                                )
                                           ]
                      ] ;
      rdfs:comment "Class representing a type of wine. The wine class is the parent class for several subclasses representing specific types of wine, including red, white, rose, sparkling, and sweet wines, as well as fortified wines." ;
      rdfs:sameAs "https://dbpedia.org/ontology/Wine"^^xsd:anyURI .


###  http://www.semanticweb.org/fnunezc/ontologies/2023/3/SpanishWineOntology#Winery
:Winery rdf:type owl:Class ;
        rdfs:comment "A class that represents a place where wine is produced, typically consisting of vineyards and a facility for winemaking." ;
        rdfs:sameAs "https://dbpedia.org/ontology/Winery"^^xsd:anyURI .


#################################################################
#    Individuals
#################################################################

###  http://www.semanticweb.org/fnunezc/ontologies/2023/3/SpanishWineOntology#Cuatro_Palmas_Amontillado
:Cuatro_Palmas_Amontillado rdf:type owl:NamedIndividual ,
                                    :OxidizingAging ;
                           :producedBy :Tio_Pepe ;
                           :hasAlcoholicContent "18.0"^^xsd:float ;
                           :hasRating "4.5"^^xsd:float .


###  http://www.semanticweb.org/fnunezc/ontologies/2023/3/SpanishWineOntology#Dos__Cortados_Palo_Cortado_Solera_Especial_Aged_20_Years
:Dos__Cortados_Palo_Cortado_Solera_Especial_Aged_20_Years rdf:type owl:NamedIndividual ,
                                                                   :OxidizingAging ;
                                                          :producedBy <http://www.semanticweb.org/fnunezc/ontologies/2023/3/SpanishWineOntology#Williams_&_Humbert> ;
                                                          :hasAlcoholicContent "18.0"^^xsd:float ;
                                                          :hasRating "4.2"^^xsd:float .


###  http://www.semanticweb.org/fnunezc/ontologies/2023/3/SpanishWineOntology#Fino_La_Barejuela
:Fino_La_Barejuela rdf:type owl:NamedIndividual ,
                            :BiologicalAgeing ;
                   :producedBy :Luis_Perez ;
                   :hasAlcoholicContent "15.0"^^xsd:float ;
                   :hasRating "4.3"^^xsd:float .


###  http://www.semanticweb.org/fnunezc/ontologies/2023/3/SpanishWineOntology#Luis_Perez
:Luis_Perez rdf:type owl:NamedIndividual ,
                     :Winery .


###  http://www.semanticweb.org/fnunezc/ontologies/2023/3/SpanishWineOntology#Tio_Pepe
:Tio_Pepe rdf:type owl:NamedIndividual ,
                   :Winery .


###  http://www.semanticweb.org/fnunezc/ontologies/2023/3/SpanishWineOntology#Williams_&_Humbert
<http://www.semanticweb.org/fnunezc/ontologies/2023/3/SpanishWineOntology#Williams_&_Humbert> rdf:type owl:NamedIndividual ,
                                                                                                       :Winery .


#################################################################
#    Rules
#################################################################

<http://www.semanticweb.org/fnunezc/ontologies/2023/3/SpanishWineOntology/fw> rdf:type <http://www.w3.org/2003/11/swrl#Variable> .

<http://www.semanticweb.org/fnunezc/ontologies/2023/3/SpanishWineOntology/alc> rdf:type <http://www.w3.org/2003/11/swrl#Variable> .

<http://www.semanticweb.org/fnunezc/ontologies/2023/3/SpanishWineOntology/wine> rdf:type <http://www.w3.org/2003/11/swrl#Variable> .

<http://www.semanticweb.org/fnunezc/ontologies/2023/3/SpanishWineOntology/time> rdf:type <http://www.w3.org/2003/11/swrl#Variable> .

[ <http://swrl.stanford.edu/ontologies/3.3/swrla.owl#isRuleEnabled> "true"^^xsd:boolean ;
   rdfs:comment "" ;
   rdfs:label "S1" ;
   rdf:type <http://www.w3.org/2003/11/swrl#Imp> ;
   <http://www.w3.org/2003/11/swrl#body> [ rdf:type <http://www.w3.org/2003/11/swrl#AtomList> ;
                                           rdf:first [ rdf:type <http://www.w3.org/2003/11/swrl#ClassAtom> ;
                                                       <http://www.w3.org/2003/11/swrl#classPredicate> :FortifiedWine ;
                                                       <http://www.w3.org/2003/11/swrl#argument1> <http://www.semanticweb.org/fnunezc/ontologies/2023/3/SpanishWineOntology/fw>
                                                     ] ;
                                           rdf:rest [ rdf:type <http://www.w3.org/2003/11/swrl#AtomList> ;
                                                      rdf:first [ rdf:type <http://www.w3.org/2003/11/swrl#DatavaluedPropertyAtom> ;
                                                                  <http://www.w3.org/2003/11/swrl#propertyPredicate> :hasAlcoholicContent ;
                                                                  <http://www.w3.org/2003/11/swrl#argument1> <http://www.semanticweb.org/fnunezc/ontologies/2023/3/SpanishWineOntology/fw> ;
                                                                  <http://www.w3.org/2003/11/swrl#argument2> <http://www.semanticweb.org/fnunezc/ontologies/2023/3/SpanishWineOntology/alc>
                                                                ] ;
                                                      rdf:rest [ rdf:type <http://www.w3.org/2003/11/swrl#AtomList> ;
                                                                 rdf:first [ rdf:type <http://www.w3.org/2003/11/swrl#BuiltinAtom> ;
                                                                             <http://www.w3.org/2003/11/swrl#builtin> <http://www.w3.org/2003/11/swrlb#lessThan> ;
                                                                             <http://www.w3.org/2003/11/swrl#arguments> [ rdf:type rdf:List ;
                                                                                                                          rdf:first <http://www.semanticweb.org/fnunezc/ontologies/2023/3/SpanishWineOntology/alc> ;
                                                                                                                          rdf:rest [ rdf:type rdf:List ;
                                                                                                                                     rdf:first 17.0 ;
                                                                                                                                     rdf:rest rdf:nil
                                                                                                                                   ]
                                                                                                                        ]
                                                                           ] ;
                                                                 rdf:rest rdf:nil
                                                               ]
                                                    ]
                                         ] ;
   <http://www.w3.org/2003/11/swrl#head> [ rdf:type <http://www.w3.org/2003/11/swrl#AtomList> ;
                                           rdf:first [ rdf:type <http://www.w3.org/2003/11/swrl#ClassAtom> ;
                                                       <http://www.w3.org/2003/11/swrl#classPredicate> :BiologicalAgeing ;
                                                       <http://www.w3.org/2003/11/swrl#argument1> <http://www.semanticweb.org/fnunezc/ontologies/2023/3/SpanishWineOntology/fw>
                                                     ] ;
                                           rdf:rest rdf:nil
                                         ]
 ] .

[ <http://swrl.stanford.edu/ontologies/3.3/swrla.owl#isRuleEnabled> "true"^^xsd:boolean ;
   rdfs:comment "" ;
   rdfs:label "S3" ;
   rdf:type <http://www.w3.org/2003/11/swrl#Imp> ;
   <http://www.w3.org/2003/11/swrl#body> [ rdf:type <http://www.w3.org/2003/11/swrl#AtomList> ;
                                           rdf:first [ rdf:type <http://www.w3.org/2003/11/swrl#ClassAtom> ;
                                                       <http://www.w3.org/2003/11/swrl#classPredicate> :BiologicalAgeing ;
                                                       <http://www.w3.org/2003/11/swrl#argument1> <http://www.semanticweb.org/fnunezc/ontologies/2023/3/SpanishWineOntology/wine>
                                                     ] ;
                                           rdf:rest [ rdf:type <http://www.w3.org/2003/11/swrl#AtomList> ;
                                                      rdf:first [ rdf:type <http://www.w3.org/2003/11/swrl#DatavaluedPropertyAtom> ;
                                                                  <http://www.w3.org/2003/11/swrl#propertyPredicate> :hasAgingTime ;
                                                                  <http://www.w3.org/2003/11/swrl#argument1> <http://www.semanticweb.org/fnunezc/ontologies/2023/3/SpanishWineOntology/wine> ;
                                                                  <http://www.w3.org/2003/11/swrl#argument2> <http://www.semanticweb.org/fnunezc/ontologies/2023/3/SpanishWineOntology/time>
                                                                ] ;
                                                      rdf:rest rdf:nil
                                                    ]
                                         ] ;
   <http://www.w3.org/2003/11/swrl#head> [ rdf:type <http://www.w3.org/2003/11/swrl#AtomList> ;
                                           rdf:first [ rdf:type <http://www.w3.org/2003/11/swrl#BuiltinAtom> ;
                                                       <http://www.w3.org/2003/11/swrl#builtin> <http://www.w3.org/2003/11/swrlb#greaterThanOrEqual> ;
                                                       <http://www.w3.org/2003/11/swrl#arguments> [ rdf:type rdf:List ;
                                                                                                    rdf:first <http://www.semanticweb.org/fnunezc/ontologies/2023/3/SpanishWineOntology/time> ;
                                                                                                    rdf:rest [ rdf:type rdf:List ;
                                                                                                               rdf:first 2 ;
                                                                                                               rdf:rest rdf:nil
                                                                                                             ]
                                                                                                  ]
                                                     ] ;
                                           rdf:rest [ rdf:type <http://www.w3.org/2003/11/swrl#AtomList> ;
                                                      rdf:first [ rdf:type <http://www.w3.org/2003/11/swrl#BuiltinAtom> ;
                                                                  <http://www.w3.org/2003/11/swrl#builtin> <http://www.w3.org/2003/11/swrlb#lessThanOrEqual> ;
                                                                  <http://www.w3.org/2003/11/swrl#arguments> [ rdf:type rdf:List ;
                                                                                                               rdf:first <http://www.semanticweb.org/fnunezc/ontologies/2023/3/SpanishWineOntology/time> ;
                                                                                                               rdf:rest [ rdf:type rdf:List ;
                                                                                                                          rdf:first 10 ;
                                                                                                                          rdf:rest rdf:nil
                                                                                                                        ]
                                                                                                             ]
                                                                ] ;
                                                      rdf:rest rdf:nil
                                                    ]
                                         ]
 ] .

[ <http://swrl.stanford.edu/ontologies/3.3/swrla.owl#isRuleEnabled> "true"^^xsd:boolean ;
   rdfs:comment "" ;
   rdfs:label "S2" ;
   rdf:type <http://www.w3.org/2003/11/swrl#Imp> ;
   <http://www.w3.org/2003/11/swrl#body> [ rdf:type <http://www.w3.org/2003/11/swrl#AtomList> ;
                                           rdf:first [ rdf:type <http://www.w3.org/2003/11/swrl#ClassAtom> ;
                                                       <http://www.w3.org/2003/11/swrl#classPredicate> :RiojaReserva ;
                                                       <http://www.w3.org/2003/11/swrl#argument1> <http://www.semanticweb.org/fnunezc/ontologies/2023/3/SpanishWineOntology/wine>
                                                     ] ;
                                           rdf:rest [ rdf:type <http://www.w3.org/2003/11/swrl#AtomList> ;
                                                      rdf:first [ rdf:type <http://www.w3.org/2003/11/swrl#DatavaluedPropertyAtom> ;
                                                                  <http://www.w3.org/2003/11/swrl#propertyPredicate> :hasAgingTime ;
                                                                  <http://www.w3.org/2003/11/swrl#argument1> <http://www.semanticweb.org/fnunezc/ontologies/2023/3/SpanishWineOntology/wine> ;
                                                                  <http://www.w3.org/2003/11/swrl#argument2> <http://www.semanticweb.org/fnunezc/ontologies/2023/3/SpanishWineOntology/time>
                                                                ] ;
                                                      rdf:rest rdf:nil
                                                    ]
                                         ] ;
   <http://www.w3.org/2003/11/swrl#head> [ rdf:type <http://www.w3.org/2003/11/swrl#AtomList> ;
                                           rdf:first [ rdf:type <http://www.w3.org/2003/11/swrl#BuiltinAtom> ;
                                                       <http://www.w3.org/2003/11/swrl#builtin> <http://www.w3.org/2003/11/swrlb#greaterThanOrEqual> ;
                                                       <http://www.w3.org/2003/11/swrl#arguments> [ rdf:type rdf:List ;
                                                                                                    rdf:first <http://www.semanticweb.org/fnunezc/ontologies/2023/3/SpanishWineOntology/time> ;
                                                                                                    rdf:rest [ rdf:type rdf:List ;
                                                                                                               rdf:first 3 ;
                                                                                                               rdf:rest rdf:nil
                                                                                                             ]
                                                                                                  ]
                                                     ] ;
                                           rdf:rest rdf:nil
                                         ]
 ] .

###  Generated by the OWL API (version 5.1.18) https://github.com/owlcs/owlapi/
